Fix EBot with .bot construction (#12)
* .bot change for substitution inside eval

* EBot simplify

engine/PrisonersDilemma/Bots/DBot.lean
@@ -7,7 +7,7 @@ namespace PDNew.Bots
 -- Bot defects if the opponent cooperates against a defect probe. --
 def DBot : Prog :=
   .ite -- If then else
-    (.sim .opp (DefectBot)) -- Simulate opponent against DefectBot
+    (.sim .opp (.bot DefectBot)) -- Simulate opponent against DefectBot
     Action.C -- test action C
     (.const Action.D) -- if opponent cooperates, defect
     (.const Action.C) -- else, cooperate
