engine/PrisonersDilemma/Bots/OBot.lean
@@ -9,10 +9,10 @@ namespace PDNew.Bots
 OBot probes the opponent's response to CooperateBot and DefectBot, and then chooses its action based on the opponent's behavior. -/
 def OBot : Prog :=
   .ite -- If then else
-    (.sim .opp (CooperateBot)) -- Simulate opponent against CooperateBot
+    (.sim .opp (.bot CooperateBot)) -- Simulate opponent against CooperateBot
     Action.C -- Test action C
     (.ite -- If opponent cooperates against CooperateBot
-      (.sim .opp (DefectBot)) -- Ask: What does opponent do against DefectBot?
+      (.sim .opp (.bot DefectBot)) -- Ask: What does opponent do against DefectBot?
       Action.C -- Test action C
       (.const Action.C) -- If opponent cooperates against DefectBot, cooperate
       (.const Action.D )) -- If opponent defects against DefectBot, defect
